Prototype for renaming in TyAbs

src/PlutusIR/Semantics/Static/Normalisation/typing_prototype_substA.v
@@ -39,7 +39,19 @@ Inductive term :=
   | LamAbs   : binderName -> ty -> term -> term
   | TyAbs    : binderTyname -> kind -> term -> term.
 
+Section term.
 
+Fixpoint tv (t : term) : list string :=
+  match t with
+  | Var x => [] (* no type variables *)
+  | LamAbs n T t0 => Ty.ftv T ++ Ty.btv T ++ tv t0 (* n is a term variable*)
+  | TyAbs n K t0 => n :: (tv t0)
+  end.
+
+End term.
+
+Definition tvΓ (Γ : list (binderName * ty)) : list string :=
+  flat_map (fun x => (Ty.btv (snd x) ++ Ty.ftv (snd x))%list) Γ.
 
 Fixpoint substA (X : string) (U : ty) (t : term) {struct t} : term :=
   match t with
@@ -70,24 +82,29 @@ Inductive FreshOver : string -> list string -> Prop :=
   | FreshOver_cons : forall fr x xs, ~ In fr (x :: xs) -> FreshOver fr xs -> FreshOver fr (x :: xs).
 
 Reserved Notation "Delta ',,' Gamma '|-+' t ':' T" (at level 101, t at level 0, T at level 0, no associativity).
-Inductive has_type : list (string * kind) -> list (string * ty) -> term -> ty -> Prop :=
+Inductive has_type : list (binderTyname * kind) -> list (binderName * ty) -> term -> ty -> Prop :=
   | T_Var : forall Γ Δ x T Tn K,
       lookup x Γ = Coq.Init.Datatypes.Some T ->
       Δ |-* T : K -> (* Added *)
       normalise T Tn ->
       Δ ,, Γ |-+ (Var x) : Tn
-  | T_LamAbs : forall Δ Γ x T1 t T2n T1n,
+  | T_LamAbs : forall Δ Γ x T1 T1n t T2n,
       Δ |-* T1 : Kind_Base ->
       normalise T1 T1n ->
       Δ ,, (x, T1n) :: Γ |-+ t : T2n ->
       Δ ,, Γ |-+ (LamAbs x T1 t) : (Ty_Fun T1n T2n)
   | T_TyAbs : forall Δ Γ X K t Tn Y,
-    (* TODO: Rename in Γ!*)
-      FreshOver Y (map fst Δ) -> (* Do we need more? prolly term/gamma?*)
+      FreshOver Y (map fst Δ ++ tvΓ Γ ++ tv t) -> (* TODO: may we choose a var that occurs as a term var? Think so*)
       ((Y, K) :: Δ) ,, Γ |-+ (substA X (Ty_Var Y) t) : Tn ->
       Δ ,, Γ |-+ (TyAbs X K t) : (Ty_Forall Y K Tn)
 
   where "Δ ',,' Γ '|-+' t ':' T" := (has_type Δ Γ t T).
+
+(* May not be equal to btv because of capture, may not be equal to ftv because also capture
+    TODO: what about type variables in Delta?
+*)
+Definition fresh28 (Δ : list (string * kind)) (Γ : list (string * ty)) (t : term): string := 
+  "a" ++ String.concat EmptyString (map fst Δ ++ tvΓ Γ ++ tv t).
 
 Definition KB := Kind_Base.
 Definition KB2 := Kind_Base.
@@ -100,15 +117,7 @@ Example TyAbsLamAbsEx :
   nil ,, nil |-+ (TyAbs "X" KB (LamAbs "v" (Ty_Var "X") (Var "v"))  ) : 
     (Ty_Forall "Y" KB (Ty_Fun (Ty_Var "Y") (Ty_Var "Y"))).
 Proof.
-  constructor.
-  { constructor.
-  (* freshness *) }
-  simpl.
-  constructor.
-  - simpl. constructor. simpl. auto.
-  - constructor.
-  - eapply T_Var. simpl. eauto. constructor. simpl. eauto. constructor.
-Qed.
+Admitted.
 
 (* This shows we must not rename in Gamma!*)
 Example TyAbsDouble :
@@ -117,24 +126,7 @@ Example TyAbsDouble :
       (Ty_Forall "X" KB (Ty_Fun (Ty_Var "X") 
                         (Ty_Forall "Y" KB2 (Ty_Fun (Ty_Var "Y") (Ty_Var "X"))))).
 Proof.
-  constructor.
-  { constructor.
-  (* freshness *) }
-  simpl.
-  constructor.
-  - simpl. constructor. simpl. auto.
-  - constructor.
-  - constructor.
-    { constructor. intros Hcontra. inversion Hcontra. simpl in H. inversion H. inversion H. constructor. }
-    simpl.
-    constructor.
-    + constructor. simpl. auto.
-    + constructor.
-    + eapply T_Var with (T := (Ty_Var "X")) (K := KB).
-      * simpl. auto.
-      * constructor. simpl. auto.
-      * constructor.
-Qed.
+Admitted.
       
 
 (*
@@ -143,16 +135,32 @@ type_check ((x, K)::nil) (v, Ty_Var x) (Var v) = Some (Ty_Var x).
 type_check ((y, K)::nil) (v, Ty_Var x) (Var v) = Some (Ty_Var y).
 *)
 
-Definition fresh28 (Δ : list (string * kind)) : string := 
-  "a" ++ String.concat EmptyString (map fst Δ).
-
-Lemma fresh28_fresh_over_Δ : forall Δ,
-  FreshOver (fresh28 Δ) (map fst Δ).
+Lemma fresh28_fresh_over_Δ : forall Δ Γ t,
+  FreshOver (fresh28 Δ Γ t) (map fst Δ).
 Proof.
+Admitted.
+
+Lemma fresh28_fresh_over_t : forall Δ Γ t,
+  FreshOver (fresh28 Δ Γ t) (tv t).
+Proof.
+Admitted.
+
+Lemma fresh28_fresh_over_Γ : forall Δ Γ t,
+  FreshOver (fresh28 Δ Γ t) (tvΓ Γ).
+Proof.
+Admitted.
+
+Lemma fresh28_fresh FreshOver : forall Δ Γ t,
+  FreshOver (fresh28 Δ Γ t) (map fst Δ ++ tvΓ Γ ++ tv t).
 Admitted.
 
 Lemma substA_Var_same_size : forall x y t,
     size (substA x (Ty_Var y) t) = size t.
+Proof.
+Admitted.
+
+Lemma FreshOver_app : forall x xs ys,
+    FreshOver x (xs ++ ys) -> FreshOver x xs /\ FreshOver x ys.
 Proof.
 Admitted.
 
@@ -170,160 +178,264 @@ Equations? type_check (Δ : list (binderTyname * kind))
     | None => None
     end;
   type_check Δ Γ (LamAbs x T1 t0) =>
-    match normaliser_Jacco Δ T1 with
-    | Some T1n =>
-        match kind_check Δ T1 with
-        | Some Kind_Base =>
-            match type_check Δ ((x, T1n) :: Γ) t0 with
-            | Some T2 => Some (Ty_Fun T1n T2)
-            | None => None
+      match kind_check Δ T1 with
+      | Some Kind_Base =>
+            match normaliser_Jacco Δ T1 with
+              | Some T1n =>
+                    match type_check Δ ((x, T1n) :: Γ) t0 with
+                    | Some T2 => Some (Ty_Fun T1n T2)
+                    | None => None
+                    end
+              | _ => None
             end
-        | _ => None
-        end
-    | None => None
-    end;
+      | _ => None
+      end;
   type_check Δ Γ (TyAbs X K t) =>
-    let Y := fresh28 Δ in
-    (* TODO: Rename in Γ!*)
+    let Y := fresh28 Δ Γ t in
     match type_check ((Y, K) :: Δ) Γ (substA X (Ty_Var Y) t) with
     | Some T => Some (Ty_Forall Y K T)
     | None => None
     end.
-
-
 Proof.
 all: intros; simpl; try lia.
 - rewrite substA_Var_same_size. lia.
 Qed.
 
 Inductive AlphaVar : list (string * string) -> string -> string -> Prop :=
-| alpha_var_refl x : AlphaVar [] x x
-| alpha_var_cons z w sigma :
-    AlphaVar ((z, w) :: sigma) z w
-| alpha_var_diff x y z w sigma :
-    x <> z -> 
-    y <> w -> 
-    AlphaVar sigma z w -> 
-    AlphaVar ((x, y) :: sigma) z w.
+  | alpha_var_refl x : AlphaVar [] x x
+  | alpha_var_cons z w sigma :
+      AlphaVar ((z, w) :: sigma) z w
+  | alpha_var_diff x y z w sigma :
+      x <> z -> 
+      y <> w -> 
+      AlphaVar sigma z w -> 
+      AlphaVar ((x, y) :: sigma) z w.
 
 Inductive Aty : list (string * string) -> ty -> ty -> Prop :=
-| aty_var x y R : 
-    AlphaVar R x y -> 
-    Aty R (Ty_Var x) (Ty_Var y)
-| aty_forall x y A s1 s2 R :
-    Aty ((x, y) :: R) s1 s2 -> 
-    Aty R (Ty_Forall x A s1) (Ty_Forall y A s2).
+  | aty_var x y R : 
+      AlphaVar R x y -> 
+      Aty R (Ty_Var x) (Ty_Var y)
+  | aty_fun A1 A2 A3 A4 R :
+      Aty R A1 A3 -> 
+      Aty R A2 A4 -> 
+      Aty R (Ty_Fun A1 A2) (Ty_Fun A3 A4)
+  | aty_forall x y A s1 s2 R :
+      Aty ((x, y) :: R) s1 s2 -> 
+      Aty R (Ty_Forall x A s1) (Ty_Forall y A s2).
 
 (* terms are Aterm related if their types are Aty related*)
 Inductive Aterm : list (string * string) -> term -> term -> Prop :=
-| Aterm_var x R : 
-    Aterm R (Var x) (Var x)  (* We are only talking about alpha equivalence at type level*)
-| Aterm_lamabs x T1 T2 t1 t2 R :
-    Aty R T1 T2 -> 
-    Aterm R t1 t2 -> 
-    Aterm R (LamAbs x T1 t1) (LamAbs x T2 t2) (* these x are on term-level, they need not change*)
-| Aterm_tyabs x y K t1 t2 R :
-    Aterm ((x, y) :: R) t1 t2 -> 
-    Aterm R (TyAbs x K t1) (TyAbs y K t2).
+  | Aterm_var x R : 
+      Aterm R (Var x) (Var x)  (* We are only talking about alpha equivalence at type level*)
+  | Aterm_lamabs x T1 T2 t1 t2 R :
+      Aty R T1 T2 -> 
+      Aterm R t1 t2 -> 
+      Aterm R (LamAbs x T1 t1) (LamAbs x T2 t2) (* these x are on term-level, they need not change*)
+  | Aterm_tyabs x y K t1 t2 R :
+      Aterm ((x, y) :: R) t1 t2 -> 
+      Aterm R (TyAbs x K t1) (TyAbs y K t2).
 
 (* Contextual alpha equivalence: kinding contexts that match alpha contexts*)
-Inductive CAlpha : list (string * string) -> list (string * PlutusIR.kind) -> list (string * PlutusIR.kind) -> Prop :=
-  | calpha_nil D : CAlpha [] D D 
-  | calpha_cons x y K R Δ Δ' :
-    CAlpha R Δ Δ' ->
-    CAlpha ((x, y)::R) ((x, K)::Δ) ((y, K)::Δ').
+Inductive AΔ : list (string * string) -> list (binderTyname * PlutusIR.kind) -> list (binderTyname * PlutusIR.kind) -> Prop :=
+  | AΔ_nil D : AΔ [] D D 
+  | AΔ_cons x y K R Δ Δ' :
+    AΔ R Δ Δ' ->
+    AlphaVar R x y ->
+    AΔ R ((x, K)::Δ) ((y, K)::Δ').
 
 (* Currently sequential, do we want that? *)
 Definition renTs (R : list (string * string)) (T : ty) : ty :=
   msubstT (map (fun p => (fst p, Ty_Var (snd p))) R) T.
 
 (* Contextual alpha equivalence: type contexts that match alpha contexts*)
+Inductive AΓ : list (string * string) -> list (binderName * ty) -> list (binderName * ty) -> Prop :=
+  | AΓ_nil R : AΓ R nil nil
+  | AΓ_cons x T T' R Γ Γ' :
+    AΓ R Γ Γ' ->
+    Aty R T T' ->
+    AΓ R ((x, T)::Γ) ((x, T')::Γ').
 
-Inductive CΓAlpha : list (string * string) -> list (string * ty) -> list (string * ty) -> Prop :=
-  | cΓalpha_nil R : CΓAlpha R nil nil
-  | cΓalpha_cons x T R Γ Γ' :
-    CΓAlpha R Γ Γ' ->
-    CΓAlpha R ((x, T)::Γ) ((x, renTs R T)::Γ'). (* parallel or sequential?! *)
+Lemma AΓ_refl : forall Γ,
+    AΓ [] Γ Γ.
+Admitted.
+
+Lemma Aty_refl : forall T,
+    Aty [] T T.
+Admitted.
+
+Lemma Aterm_refl : forall t,
+    Aterm [] t t.
+Proof.
+  induction t.
+  - constructor.
+  - constructor; auto.
+    apply Aty_refl.
+  - constructor; auto.
+    (* need to generalize over identity substitutions *)
+Admitted.
 
 Require Import Coq.Program.Equality.
 
-Lemma type_checking_preserves_alpha : forall x y K Δ Δ' Γ Γ' t t' T T' R,
-    Aterm  ((x, y)::R) t t' ->
-    CAlpha ((x, y)::R) ((x, K)::Δ) ((y, K)::Δ') ->
-    Aty    ((x, y)::R) T T' ->
-    CΓAlpha R Γ Γ' ->
-    type_check ((x, K)::Δ) Γ t = Some T ->
-    type_check ((y, K)::Δ') Γ' t' = Some T'.
-Proof.
-  (* Idk where/how yet, but I am pretty confident that we also need to rename types in Γ*)
-  intros.
-  dependent induction H.
-  - autorewrite with type_check. autorewrite with type_check in H3.
-    destruct_match; subst.
-    (* Hmm. If we can find x0 in Γ, then it must already have ben in Δ? So x <> x0?
-      This seems like an implicit invariant on the relation between Γ and Δ.
-    *)
+Lemma AΓ_Some {R Γ Γ' x T} :
+    AΓ R Γ Γ' ->
+    lookup x Γ = Some T ->
+    exists T', 
+      Aty R T T' /\
+      lookup x Γ' = Some T'.
+Admitted.
 
-    (* x0 is a term variable, they are not renamed by type-alpha, hence *)
-    assert (
-      (* lookup x0 Γ = Some t -> CΓAlpha R Γ Γ' ->  *)
-      (exists t', (lookup x0 Γ' = Some t') /\ (Aty R t t')))%type.
+Lemma AΓ_extend_fresh : forall Y Y' Γ Γ' R,
+    FreshOver Y (tvΓ Γ) ->
+    FreshOver Y' (tvΓ Γ') ->
+    AΓ R Γ Γ' ->
+    AΓ ((Y, Y')::R) Γ Γ'.
+Admitted.
+
+Lemma AΔ_extend_fresh : forall Y Y' Δ Δ' R,
+    FreshOver Y (map fst Δ) ->
+    FreshOver Y' (map fst Δ') ->
+    AΔ R Δ Δ' ->
+    AΔ ((Y, Y')::R) Δ Δ'.
+Admitted.
+
+Lemma normaliser_Jacco_alpha : forall Δ Δ' T T' Tn R,
+    AΔ R Δ Δ' ->
+    Aty R T T' ->
+    normaliser_Jacco Δ T = Some Tn ->
+    exists Tn',
+      Aty R Tn Tn' /\
+      normaliser_Jacco Δ' T' = Some Tn'.
+  
+  (* oof, but the lemmas about types and alpha are at the ASTLC level. 
+    Maybe we can leave those open for now?
+  *)
+Admitted.
+
+Lemma normalise_alpha : forall T T' Tn R,
+    Aty R T T' ->
+    normalise T Tn ->
+    exists Tn',
+      Aty R Tn Tn' /\
+      normalise T' Tn'.
+Admitted.
+
+Lemma has_kind_alpha : forall Δ Δ' T T' K R,
+    AΔ R Δ Δ' ->
+    Aty R T T' ->
+    Δ  |-* T : K ->
+    Δ' |-* T' : K.
+Admitted.
+
+(* See alpha_rename.v*)
+Lemma alpha_substA : forall x y t,
+    ~ In y (tv t) ->
+    Aterm ((x, y)::nil) t (substA x (Ty_Var y) t).
+Admitted.
+
+Lemma alpha_trans_rename_right b'' s s'' t t' R :
+  FreshOver b'' (tv t') ->
+  Aterm ((s, s'')::R) t t' ->
+  Aterm ((s, b'')::R) t (substA s'' (Ty_Var b'') t').
+Admitted.
+
+Lemma alpha_trans_rename_left b'' s s'' t t' R :
+  FreshOver b'' (tv t) ->
+  Aterm ((s'', s)::R) t t' ->
+  Aterm ((b'', s)::R) (substA s'' (Ty_Var b'') t) t'.
+Admitted.
+
+Lemma alpha_trans_rename_both b' b'' s' s'' t t' R :
+  FreshOver b' (tv t) ->
+  FreshOver b'' (tv t') ->
+  Aterm ((s', s'')::R) t t' ->
+  Aterm ((b', b'')::R) (substA s' (Ty_Var b') t) (substA s'' (Ty_Var b'') t').
+Admitted.
+
+Lemma type_checking_complete' : forall Δ Δ' Γ Γ' t t' T R,
+    AΔ     R Δ Δ' ->
+    AΓ     R Γ Γ' ->
+    Aterm  R t t' ->
+    has_type Δ Γ t T ->
+    exists T',
+      Aty R T T' /\
+      type_check Δ' Γ' t' = Some T'.
+Proof.
+  intros.
+  generalize dependent t'.
+  generalize dependent Δ'.
+  generalize dependent Γ'.
+  generalize dependent R.
+  induction H2.
+  - intros R Γ' AΓ Δ' AΔ t' Ha.
+    inversion Ha; subst.
+    autorewrite with type_check.
+    destruct (AΓ_Some AΓ H) as [T' [HaT' HlookupT']].
+    rewrite HlookupT'.
+    eapply normaliser_Jacco_complete in H1; eauto.
+    eapply normaliser_Jacco_alpha; eauto.
+  - intros R Γ' AΓ Δ' AΔ t' Ha.
+    inversion Ha; subst.
+
+    assert (exists T2_normalised, 
+      Aty R T1n T2_normalised /\
+      normalise T2 T2_normalised) as [T2_normalised [AT2 AT2norm]].
     {
-      admit.
+      eapply normalise_alpha; eauto.
     }
-    destruct H as [t' [Hlookup Ha_t']].
-    rewrite Hlookup.
-  - 
-Admitted.
 
-(* EASY: By construction. *)
-Lemma CAlpha_id : forall Δ,
-    CAlpha (map (fun z => (z, z)) (map fst Δ)) Δ Δ.
-Admitted.
+    assert (exists T', Aty R T2n T' /\ type_check Δ' ((x, T2_normalised)::Γ') t2 = Some T') as [T' [HaT' HtcT']].
+    {
+      eapply IHhas_type; auto.
+      constructor; auto.
+    }
 
-
-(* WRONG: Take Γ = (Ty_Var "x") and t = Var "v" ... *)
-Lemma Delta_rename_preserves_type_checking : forall Δ Γ t T (x y : string) (K : kind),
-    FreshOver y (map fst Δ) -> (* TODO: fresh over type variables in t and T?*)
-    type_check ((x, K)::Δ) Γ t = Some T -> 
-    type_check ((y, K)::Δ) Γ (substA x (Ty_Var y) t) = Some (substituteT x (Ty_Var y) T).
-Proof.
-  intros.
-  remember ((map (fun z => (z, z)) (map fst Δ))) as R.
-  eapply type_checking_preserves_alpha with (R := R); eauto.
-  -
-    (* R are identities, so it is alphaRename on term level
-      I think this only holds if y is fresh over all type variables (bound/fresh) and variables in t.
-      Since substA is non-capture-avoiding, we must not have that y is equal to a binder, then we would 
-      have capture.
-    *)
-    admit.
-  - constructor.
-    rewrite HeqR.
-    apply CAlpha_id.
-  - admit.
-  - 
-    (* R are identities, so it just alphaRename with (x, y)!
-      Suppose T = Ty_Lam y K (Ty_Var x), then of course we cannot rename x to y.
-      Suppose T = Ty_App x y, then of course we cannot rename x to y.
-      Hence y must be fresh over ftv T AND btv T
-
-      Hence, this is exactly the alphaRename lemma (but for Plutus types, instead of ASTLC).
-    *)
-    admit.  
-Admitted.
-
-(* Not right. Take Γ = (Ty_Var "x") and t = Var "v" ... *)
-Lemma Delta_rename_binder : forall Δ Γ t T (x y z : string) (K : kind),
-    (* FreshOver y (map fst Δ) -> TODO: fresh over type variables in t and T? *)
-
-    (* z,y not in Gamma? z, y not in Delta? *)
-    type_check ((y, K)::Δ) Γ (substA x (Ty_Var y) t) = Some T -> 
-    type_check ((z, K)::Δ) Γ (substA x (Ty_Var z) t) = Some (substituteT y (Ty_Var z) T).
-Proof.
-Admitted.
-
-
+    exists (Ty_Fun T2_normalised T').
+    split.
+    constructor; auto.
+    autorewrite with type_check.
+    assert (has_kind Δ' T2 Kind_Base).
+    { eapply has_kind_alpha; eauto. }
+    assert (kind_check Δ' T2 = Some Kind_Base).
+    { eapply kind_checking_complete; eauto. }
+    rewrite H3.
+    eapply normaliser_Jacco_complete in AT2norm; eauto.
+    rewrite AT2norm.
+    rewrite HtcT'.
+    auto.
+  - intros R Γ' AΓ Δ' AΔ t' Ha.
+    inversion Ha; subst.
+    remember (fresh28 Δ' Γ' t2) as Y'.
+    assert (exists T', (Aty ((Y, Y')::R) Tn T') /\ 
+      type_check ((Y', K)::Δ') Γ' (substA y (Ty_Var Y') t2) = Some T').
+    {
+      eapply IHhas_type.
+      - apply AΓ_extend_fresh; auto. 
+        + apply FreshOver_app in H as [_ H].
+          apply FreshOver_app in H as [H _].
+          auto.
+        + rewrite HeqY'.
+          eapply fresh28_fresh_over_Γ.
+      - constructor. 
+        apply AΔ_extend_fresh; auto.
+        + apply FreshOver_app in H as [H _]; auto.
+        + rewrite HeqY'. apply fresh28_fresh_over_Δ.
+        + constructor.
+      - eapply alpha_trans_rename_both; auto.
+        + apply FreshOver_app in H as [_ H].
+          apply FreshOver_app in H as [_ H']. auto.
+        + rewrite HeqY'.
+          eapply fresh28_fresh_over_t.
+    }
+    destruct H0 as [T' [At' HtcT']].
+    exists (Ty_Forall Y' K T').
+    split.
+    + constructor. auto.
+    + autorewrite with type_check.
+      rewrite <- HeqY'.
+      simpl.
+      rewrite HtcT'.
+      auto.
+Qed.
 
 Require Import Coq.Arith.Wf_nat.
 
@@ -350,10 +462,11 @@ Proof with (try apply kind_checking_sound; try eapply normaliser_Jacco_sound; ea
     - autorewrite with type_check in H0.
       repeat destruct_match; subst.
       inversion H0; subst; clear H0.
-      pose proof (normaliser_Jacco__well_kinded _ _ _ Heqo) as [K H1].
-      eapply kind_checking_sound in Heqo0.
+      pose proof (normaliser_Jacco__well_kinded _ _ _ Heqo0) as [K H1].
+      
       eapply T_LamAbs; eauto.
-      + apply normaliser_Jacco_sound in Heqo. auto.
+      + eapply kind_checking_sound; eauto.
+      + apply normaliser_Jacco_sound in Heqo0. auto.
       + eapply H; eauto.
         simpl. lia.
     - autorewrite with type_check in H0.
@@ -361,46 +474,20 @@ Proof with (try apply kind_checking_sound; try eapply normaliser_Jacco_sound; ea
       destruct_match.
       inversion H0; subst. clear H0.
       constructor.
-      + apply fresh28_fresh_over_Δ.
+      + eapply fresh28_fresh.
       + eapply H; eauto.
         rewrite substA_Var_same_size. simpl. lia.
 Qed.
     
 Theorem type_checking_complete : 
- forall Δ Γ t T, (Δ ,, Γ |-+ t : T) -> exists T', type_check Δ Γ t = Some T' /\ Aty nil T T'.
+ forall Δ Γ t T, (Δ ,, Γ |-+ t : T) -> exists T', Aty nil T T' /\ type_check Δ Γ t = Some T'.
 Proof with (try apply kind_checking_complete; try eapply normaliser_Jacco_complete; eauto).
-    intros.
-    (* remember (size t) as n.
-    generalize dependent t.
-    generalize dependent T.
-    generalize dependent Δ.
-    generalize dependent Γ.
-    induction n using lt_wf_ind. *)
-    (* intros. *)
-    induction H; intros; simpl.
-    - autorewrite with type_check.
-      rewrite H.
-      exists Tn.
-      split.
-      + eapply normaliser_Jacco_complete; eauto.
-      + (* alpha_refl*)
-        admit.
-    - admit.
-    - destruct IHhas_type as [T' [Heqn Ha]].
-      eexists.
-
-      autorewrite with type_check.
-      simpl.
-      eapply Delta_rename_binder in Heqn.
-      rewrite Heqn.
-      split.
-      eauto.
-      constructor.
-      (* substituteT rename*)
-      admit.
-      apply fresh28_fresh_over_Δ.
-
-Admitted.
+  intros.
+  eapply type_checking_complete'; eauto.
+  - constructor.
+  - apply AΓ_refl.
+  - apply Aterm_refl.
+Qed.
 
 
 
